tests/lean/run/subst_vars.lean
@@ -1,0 +1,4 @@
+open tactic
+
+example (a b c d : nat) : a = b → b = c → d = c → a = d :=
+by intros; subst_vars
